\chapter{Operatoren}
\section{Lie-Ableitung}
Es gilt:
\begin{equation}
    L_f^i h(x) = \frac{\partial L_f^{i-1} h(x)}{\partial x} f(x)
\end{equation}
au√üerdem gilt:
\begin{equation}
    L_f^0 h(x) = h(x)
\end{equation}

\section{Lie-Klammern}
Es gilt:
\begin{equation}
    [\tau_1(x), \tau_2(x)] = \frac{\partial \tau_2(x)}{\partial x} \tau_1(x) - \frac{\partial \tau_1(x)}{\partial x} \tau_2(x)
\end{equation}

\section{Zusammenhang zwischen Lie-Ableitungen und Lie-Klammern}
Es gilt:
\begin{equation}
    L_{ad_f g(x)} h(x) = L_f L_g h(x) - L_g L_f h(x)
\end{equation}
mit
\begin{equation}
    ad_f g(x) = [f(x), g(x)]
\end{equation}
und
\begin{equation}
    ad_f^k g(x) = ad_f (ad_f^{k-1} g(x))
\end{equation}
sowie
\begin{equation}
    ad_f^0 g(x) = g(x)
\end{equation}

\section{$M_A$-Operator}
Es gilt:
\begin{equation}
    M_A c^\text{T} (t) = c^\text{T} (t) A(t) + \dot{c}^\text{T} (t)
\end{equation}

\section{$N_A$-Operator}
Es gilt:
\begin{equation}
    N_A s^1(t) = A(t) s^1(t) - \dot{s}^1(t)
\end{equation}

